@prefix c4p: <http://c4p.org/1/> .
@prefix rdf: <http://www.w3.org/1999/02/22-rdf-syntax-ns#> .
@prefix skos: <http://www.w3.org/2004/02/skos/core#> .

c4p:atmosphericSciences rdf:type skos:Concept ; 
	skos:prefLabel   "atmosphericSciences"  ; 
	skos:narrower   c4p:aerosols  ; 
	skos:narrower   c4p:atmosphericChemistry  ; 
	skos:narrower   c4p:atmosphericDynamics  ; 
	skos:narrower   c4p:atmosphericPhysics  ; 
	skos:narrower   c4p:environmentalSciences  ; 
	skos:narrower   c4p:isotopicGeology  ; 
	skos:narrower   c4p:meteorology  ; 
	skos:narrower   c4p:nephology  ; 
	skos:definition   "an umbrella term for the study of the atmosphere, its processes, the effects other systems have on the atmosphere, and the effects of the atmosphere on these other systems. Meteorology includes atmospheric chemistry and atmospheric physics with a major focus on weather forecasting. Climatology is the study of atmospheric changes (both long and short-term) that define average climates and their change over time, due to both natural and anthropogenic climate variability. Aeronomy is the study of the upper layers of the atmosphere, where dissociation and ionization are important. Atmospheric science has been extended to the field of planetary science and the study of the atmospheres of the planets of the solar system."  . 

c4p:climatology rdf:type skos:Concept ; 
	skos:prefLabel   "climatology"  ; 
	skos:narrower   c4p:dendrochronology  ; 
	skos:narrower   c4p:glacialGeology  ; 
	skos:narrower   c4p:lacustrineSedimentology  ; 
	skos:narrower   c4p:limnology  ; 
	skos:narrower   c4p:palynology  ; 
	skos:narrower   c4p:paleoenvironment  ; 
	skos:narrower   c4p:paleofire  ; 
	skos:definition   "the study of climate, scientifically defined as weather conditions averaged over a period of time."  . 

c4p:cryology rdf:type skos:Concept ; 
	skos:prefLabel   "cryology"  ; 
	skos:narrower   c4p:polar  ; 
	skos:narrower   c4p:glacialGeology  ; 
	skos:narrower   c4p:glaciology  ; 
	skos:narrower   c4p:glacialGeomorphology  ; 
	skos:narrower   c4p:permafrost  ; 
	skos:definition   " the study of snow and ice."  . 

c4p:geobiology rdf:type skos:Concept ; 
	skos:prefLabel   "geobiology"  ; 
	skos:narrower   c4p:archaeology  ; 
	skos:narrower   c4p:anthropology  ; 
	skos:narrower   c4p:biodiversity  ; 
	skos:narrower   c4p:biogeography  ; 
	skos:narrower   c4p:botany  ; 
	skos:narrower   c4p:dendrochronology  ; 
	skos:narrower   c4p:developmentalBiologyEmbryology  ; 
	skos:narrower   c4p:ecology  ; 
	skos:narrower   c4p:entomology  ; 
	skos:narrower   c4p:environmentalScience  ; 
	skos:narrower   c4p:evolutionaryBiology  ; 
	skos:narrower   c4p:forestry  ; 
	skos:narrower   c4p:ichthyology  ; 
	skos:narrower   c4p:invertebrate  ; 
	skos:narrower   c4p:molecularBiology  ; 
	skos:narrower   c4p:organismalBiology  ; 
	skos:narrower   c4p:phylogenetics  ; 
	skos:narrower   c4p:planktology  ; 
	skos:narrower   c4p:taxonomy  ; 
	skos:narrower   c4p:vertebrate  ; 
	skos:narrower   c4p:zoology  ; 
	skos:definition   " an interdisciplinary field of scientific research that explores interactions between the biosphere and the lithosphere and/or the atmosphere."  . 

c4p:geochemistry rdf:type skos:Concept ; 
	skos:prefLabel   "geochemistry"  ; 
	skos:narrower   c4p:agrogeology  ; 
	skos:narrower   c4p:aqueousGeochemistry  ; 
	skos:narrower   c4p:biogeochemistry  ; 
	skos:narrower   c4p:cosmochemistry  ; 
	skos:narrower   c4p:explorationGeochemistry  ; 
	skos:narrower   c4p:forensicGeochemistry  ; 
	skos:narrower   c4p:geochemistry  ; 
	skos:narrower   c4p:isotopicGeochemistry  ; 
	skos:narrower   c4p:petroleumGeochemistry  ; 
	skos:narrower   c4p:regionalGeochemistry  ; 
	skos:narrower   c4p:terrestrialGeochemistry  ; 
	skos:definition   "is the science that uses the tools and principles of chemistry to explain the mechanisms behind major geological systems such as the Earth's crust and its oceans"  . 

c4p:geochronology rdf:type skos:Concept ; 
	skos:prefLabel   "geochronology"  ; 
	skos:narrower   c4p:absoluteDating  ; 
	skos:narrower   c4p:biostratigraphy  ; 
	skos:narrower   c4p:chronostratigraphy  ; 
	skos:narrower   c4p:geochronology  ; 
	skos:narrower   c4p:geochronometry  ; 
	skos:narrower   c4p:geologicTime  ; 
	skos:narrower   c4p:historicalGeology  ; 
	skos:narrower   c4p:isotopicGeochronology  ; 
	skos:narrower   c4p:lithostratigraphy  ; 
	skos:narrower   c4p:relativeDating  ; 
	skos:definition   "is the science of determining the age of rocks, fossils, and sediments, within a certain degree of uncertainty inherent to the method used."  . 

c4p:geoinformatics rdf:type skos:Concept ; 
	skos:prefLabel   "geoinformatics"  ; 
	skos:narrower   c4p:cartography  ; 
	skos:narrower   c4p:dataManipulation  ; 
	skos:narrower   c4p:forcasting  ; 
	skos:narrower   c4p:geography  ; 
	skos:narrower   c4p:geologicMapping  ; 
	skos:narrower   c4p:geomodeling  ; 
	skos:narrower   c4p:gIS  ; 
	skos:narrower   c4p:graphing  ; 
	skos:narrower   c4p:lIDAR  ; 
	skos:narrower   c4p:mapping  ; 
	skos:narrower   c4p:metadata  ; 
	skos:narrower   c4p:modelling  ; 
	skos:narrower   c4p:satellite  ; 
	skos:narrower   c4p:statisticalAnalysis  ; 
	skos:narrower   c4p:visualization  ; 
	skos:definition   "is the science and the technology which develops and uses information science infrastructure to address the problems of geography, geosciences and related branches of engineering."  . 

c4p:hydrology rdf:type skos:Concept ; 
	skos:prefLabel   "hydrology"  ; 
	skos:narrower   c4p:geohydrology  ; 
	skos:narrower   c4p:hydrogeology  ; 
	skos:narrower   c4p:hydrology  ; 
	skos:narrower   c4p:lacustrine  ; 
	skos:narrower   c4p:limnogeology  ; 
	skos:narrower   c4p:limnology  ; 
	skos:definition   "is the science and the technology which develops and uses information science infrastructure to address the problems of geography, geosciences and related branches of engineering."  . 

c4p:oceanography rdf:type skos:Concept ; 
	skos:prefLabel   "oceanography"  ; 
	skos:narrower   c4p:bathymetry  ; 
	skos:narrower   c4p:deepSeaResearch  ; 
	skos:narrower   c4p:marineGeoscience  ; 
	skos:narrower   c4p:paleobathymetry  ; 
	skos:narrower   c4p:paleoceanography  ; 
	skos:narrower   c4p:paleomagnetism  ; 
	skos:narrower   c4p:oceanography  ; 
	skos:definition   "branch of Earth science that studies the ocean. It covers a wide range of topics, including marine organisms and ecosystem dynamics; ocean currents, waves, and geophysical fluid dynamics; plate tectonics and the geology of the sea floor; and fluxes of various chemical substances and physical properties within the ocean and across its boundaries."  . 

c4p:paleobiology rdf:type skos:Concept ; 
	skos:prefLabel   "paleobiology"  ; 
	skos:narrower   c4p:biofacies  ; 
	skos:narrower   c4p:biostratinomy  ; 
	skos:narrower   c4p:calcareousNannofossil  ; 
	skos:narrower   c4p:fossilization  ; 
	skos:narrower   c4p:invertebrate  ; 
	skos:narrower   c4p:vertebrate  ; 
	skos:narrower   c4p:geoarcheology  ; 
	skos:narrower   c4p:ichnology  ; 
	skos:narrower   c4p:mammalPaleobiology  ; 
	skos:narrower   c4p:microfossil  ; 
	skos:narrower   c4p:micropaleobiology  ; 
	skos:narrower   c4p:morphology  ; 
	skos:narrower   c4p:paleobiogeography  ; 
	skos:narrower   c4p:paleobiology  ; 
	skos:narrower   c4p:paleobotany  ; 
	skos:narrower   c4p:paleoecology  ; 
	skos:narrower   c4p:paleoentomology  ; 
	skos:narrower   c4p:paleofire  ; 
	skos:narrower   c4p:paleoichthyology  ; 
	skos:narrower   c4p:paleontology  ; 
	skos:narrower   c4p:paleozoology  ; 
	skos:narrower   c4p:palynology  ; 
	skos:narrower   c4p:taphonomy  ; 
	skos:definition   "combines the methods and findings of the natural science biology with the methods and findings of the earth science paleontology. It is occasionally referred to as geobiology."  . 

c4p:physicalGeology rdf:type skos:Concept ; 
	skos:prefLabel   "physicalGeology"  ; 
	skos:narrower   c4p:drilling  ; 
	skos:narrower   c4p:economicGeology  ; 
	skos:narrower   c4p:energyResources  ; 
	skos:narrower   c4p:geodesy  ; 
	skos:narrower   c4p:engineeringGeology  ; 
	skos:narrower   c4p:geophysics  ; 
	skos:narrower   c4p:mineralogy  ; 
	skos:narrower   c4p:miningGeology  ; 
	skos:narrower   c4p:naturalResources  ; 
	skos:narrower   c4p:ore  ; 
	skos:narrower   c4p:petroleumGeology  ; 
	skos:narrower   c4p:petrology  ; 
	skos:narrower   c4p:petrophysics  ; 
	skos:narrower   c4p:seismology  ; 
	skos:narrower   c4p:subsurfaceExploration  ; 
	skos:narrower   c4p:tectonics  ; 
	skos:definition   "That branch of geology concerned with understanding the composition of the earth and the physical changes occurring in it, based on the study of rocks, minerals, and sediments, their structures and formations, and their processes of origin and alteration."  . 

c4p:sedimentology rdf:type skos:Concept ; 
	skos:prefLabel   "sedimentology"  ; 
	skos:narrower   c4p:coastalSedimentology  ; 
	skos:narrower   c4p:edaphology  ; 
	skos:narrower   c4p:paleomagnetism  ; 
	skos:narrower   c4p:pedology  ; 
	skos:narrower   c4p:relativeDating  ; 
	skos:narrower   c4p:sedimentology  ; 
	skos:narrower   c4p:stratigraphy  ; 
	skos:definition   "The science concerned with the description, classification, origin, and interpretation of sediments and sedimentary rock."  . 

c4p:aerosols rdf:type skos:Concept ; 
	skos:prefLabel   "aerosols"  ; 
	skos:definition   "a suspension of fine solid or liquid particles in gas"  . 

c4p:atmosphericChemistry rdf:type skos:Concept ; 
	skos:prefLabel   "atmosphericChemistry"  ; 
	skos:definition   "The study of the production, transport, modification, and removal of atmospheric constituents in the troposphere and stratosphere."  . 

c4p:atmosphericDynamics rdf:type skos:Concept ; 
	skos:prefLabel   "atmosphericDynamics"  ; 
	skos:definition   "The study of the dynamic phenomena of the atmosphere."  . 

c4p:atmosphericPhysics rdf:type skos:Concept ; 
	skos:prefLabel   "atmosphericPhysics"  ; 
	skos:definition   "The study of the physical phenomena of the atmosphere."  . 

c4p:environmentalSciences rdf:type skos:Concept ; 
	skos:prefLabel   "environmentalSciences"  ; 
	skos:definition   "the branch of biology concerned with the relations between organisms and their environment"  . 

c4p:isotopicGeology rdf:type skos:Concept ; 
	skos:prefLabel   "isotopicGeology"  ; 
	skos:definition   "an aspect of geology based upon study of the natural variations in the relative abundances of isotopes of various elements."  . 

c4p:meteorology rdf:type skos:Concept ; 
	skos:prefLabel   "meteorology"  ; 
	skos:definition   "the branch of science concerned with the processes and phenomena of the atmosphere, especially as a means of forecasting the weather"  . 

c4p:nephology rdf:type skos:Concept ; 
	skos:prefLabel   "nephology"  ; 
	skos:definition   "the study or contemplation of clouds"  . 

c4p:dendrochronology rdf:type skos:Concept ; 
	skos:prefLabel   "dendrochronology"  ; 
	skos:definition   "the science or technique of dating events, environmental change, and archaeological artifacts by using the characteristic patterns of annual growth rings in timber and tree trunks"  . 

c4p:glacialGeology rdf:type skos:Concept ; 
	skos:prefLabel   "glacialGeology"  ; 
	skos:definition   "the study of glaciers, or more generally ice and natural phenomena that involve ice"  . 

c4p:lacustrineSedimentology rdf:type skos:Concept ; 
	skos:prefLabel   "lacustrineSedimentology"  ; 
	skos:definition   "of, relating to, or associated with lakes and the physical and chemical properties of sedimentary rocks and the processes involved in their formation, including transportation, deposition, and lithification of sediments"  . 

c4p:limnology rdf:type skos:Concept ; 
	skos:prefLabel   "limnology"  ; 
	skos:definition   "the study of the biological, chemical, and physical features of lakes and other bodies of fresh water"  . 

c4p:palynology rdf:type skos:Concept ; 
	skos:prefLabel   "palynology"  ; 
	skos:definition   "the study of pollen grains and other spores, especially as found in archaeological or geological deposits"  . 

c4p:paleoenvironment rdf:type skos:Concept ; 
	skos:prefLabel   "paleoenvironment"  ; 
	skos:definition   "an environment prevailing at a particular time in the geological past"  . 

c4p:paleofire rdf:type skos:Concept ; 
	skos:prefLabel   "paleofire"  ; 
	skos:definition   "the study of ancient fire "  . 

c4p:polar rdf:type skos:Concept ; 
	skos:prefLabel   "polar"  ; 
	skos:definition   "of or relating to the North or South Pole"  . 

c4p:glacialGeology rdf:type skos:Concept ; 
	skos:prefLabel   "glacialGeology"  ; 
	skos:definition   "Glaciology is the study of glaciers, or more generally ice and natural phenomena that involve ice"  . 

c4p:glaciology rdf:type skos:Concept ; 
	skos:prefLabel   "glaciology"  ; 
	skos:definition   "Glaciology is an interdisciplinary earth science that integrates geophysics, geology, physical geography, geomorphology, climatology, meteorology, hydrology, biology, and ecology."  . 

c4p:glacialGeomorphology rdf:type skos:Concept ; 
	skos:prefLabel   "glacialGeomorphology"  ; 
	skos:definition   "the study of the physical features of the surface of ice and their relation to its geological structures"  . 

c4p:permafrost rdf:type skos:Concept ; 
	skos:prefLabel   "permafrost"  ; 
	skos:definition   "a thick subsurface layer of soil that remains frozen throughout the year, occurring chiefly in polar regions"  . 

c4p:archaeology rdf:type skos:Concept ; 
	skos:prefLabel   "archaeology"  ; 
	skos:definition   "the study of human history and prehistory through the excavation of sites and the analysis of artifacts and other physical remains"  . 

c4p:anthropology rdf:type skos:Concept ; 
	skos:prefLabel   "anthropology"  ; 
	skos:definition   "the study of humankind"  . 

c4p:biodiversity rdf:type skos:Concept ; 
	skos:prefLabel   "biodiversity"  ; 
	skos:definition   "the variety of life in the world or in a particular habitat or ecosystem"  . 

c4p:biogeography rdf:type skos:Concept ; 
	skos:prefLabel   "biogeography"  ; 
	skos:definition   "the branch of biology that deals with the geographical distribution of plants and animals"  . 

c4p:botany rdf:type skos:Concept ; 
	skos:prefLabel   "botany"  ; 
	skos:definition   "the scientific study of plants, including their physiology, structure, genetics, ecology, distribution, classification, and economic importance"  . 

c4p:dendrochronology rdf:type skos:Concept ; 
	skos:prefLabel   "dendrochronology"  ; 
	skos:definition   "the science or technique of dating events, environmental change, and archaeological artifacts by using the characteristic patterns of annual growth rings in timber and tree trunks"  . 

c4p:developmentalBiologyEmbryology rdf:type skos:Concept ; 
	skos:prefLabel   "developmentalBiologyEmbryology"  ; 
	skos:definition   " the study of the process by which organs grow and develop, and is closely related to Ontogeny"  . 

c4p:ecology rdf:type skos:Concept ; 
	skos:prefLabel   "ecology"  ; 
	skos:definition   "the branch of biology that deals with the relations of organisms to one another and to their physical surroundings."  . 

c4p:entomology rdf:type skos:Concept ; 
	skos:prefLabel   "entomology"  ; 
	skos:definition   "the branch of zoology concerned with the study of insects"  . 

c4p:environmentalScience rdf:type skos:Concept ; 
	skos:prefLabel   "environmentalScience"  ; 
	skos:definition   "the science of the interactions between the physical, chemical, and biological components of the environment, including their effects on all types of organisms but more often refers to human impact on the environment."  . 

c4p:evolutionaryBiology rdf:type skos:Concept ; 
	skos:prefLabel   "evolutionaryBiology"  ; 
	skos:definition   "Biological evolution, simply put, is descent with modification. Thisdefinition encompasses small-scale evolution (changes in gene frequency in a population from one generation to the next) and large-scaleevolution (the descent of different species from a common ancestor over many generations)."  . 

c4p:forestry rdf:type skos:Concept ; 
	skos:prefLabel   "forestry"  ; 
	skos:definition   "the science or practice of planting, managing, and caring for forests"  . 

c4p:ichthyology rdf:type skos:Concept ; 
	skos:prefLabel   "ichthyology"  ; 
	skos:definition   "the branch of zoology that deals with fishes"  . 

c4p:invertebrate rdf:type skos:Concept ; 
	skos:prefLabel   "invertebrate"  ; 
	skos:definition   "an animal lacking a backbone, such as an arthropod, mollusk, annelid, coelenterate, etc. The invertebrates constitute an artificial division of the animal kingdom, comprising 95 percent of animal species and about 30 different phyla"  . 

c4p:molecularBiology rdf:type skos:Concept ; 
	skos:prefLabel   "molecularBiology"  ; 
	skos:definition   " the branch of biology that deals with the molecular basis of biological activity. This field overlaps with other areas of biology and chemistry, particularly genetics and biochemistry."  . 

c4p:organismalBiology rdf:type skos:Concept ; 
	skos:prefLabel   "organismalBiology"  ; 
	skos:definition   "the study of structure, function, ecology and evolution at the level of the organism, provides a rich arena for investigation on its own, but also plays a central role in answering conceptual questions about both ecology and evolution. "  . 

c4p:phylogenetics rdf:type skos:Concept ; 
	skos:prefLabel   "phylogenetics"  ; 
	skos:definition   " the study of evolutionary relationships among groups of organisms (e.g. species, populations), which are discovered through molecular sequencing data and morphological data matrices."  . 

c4p:planktology rdf:type skos:Concept ; 
	skos:prefLabel   "planktology"  ; 
	skos:definition   " the study of plankton, various small drifting plants, animals and microorganisms that inhabit bodies of water. The field encompasses a variety of topics, including primary production and energy flow."  . 

c4p:taxonomy rdf:type skos:Concept ; 
	skos:prefLabel   "taxonomy"  ; 
	skos:definition   "the branch of science concerned with classification, especially of organisms; systematics."  . 

c4p:vertebrate rdf:type skos:Concept ; 
	skos:prefLabel   "vertebrate"  ; 
	skos:definition   "an animal of a large group distinguished by the possession of a backbone or spinal column, including mammals, birds, reptiles, amphibians, and fishes"  . 

c4p:zoology rdf:type skos:Concept ; 
	skos:prefLabel   "zoology"  ; 
	skos:definition   "the scientific study of the behavior, structure, physiology, classification, and distribution of animals"  . 

c4p:agrogeology rdf:type skos:Concept ; 
	skos:prefLabel   "agrogeology"  ; 
	skos:definition   "the branch of geology concerned with the adaptability of land to agriculture, soil quality, etc. "  . 

c4p:aqueousGeochemistry rdf:type skos:Concept ; 
	skos:prefLabel   "aqueousGeochemistry"  ; 
	skos:definition   "the study of the chemical composition of the earth and its rocks and minerals, with a focus on water"  . 

c4p:biogeochemistry rdf:type skos:Concept ; 
	skos:prefLabel   "biogeochemistry"  ; 
	skos:definition   " the scientific discipline that involves the study of the chemical, physical, geological, and biological processes and reactions that govern the composition of the natural environment (including the biosphere, the cryosphere, the hydrosphere, the pedosphere, the atmosphere, and the lithosphere)."  . 

c4p:cosmochemistry rdf:type skos:Concept ; 
	skos:prefLabel   "cosmochemistry"  ; 
	skos:definition   "the science dealing with the occurrence and distribution of chemical elements in the universe"  . 

c4p:explorationGeochemistry rdf:type skos:Concept ; 
	skos:prefLabel   "explorationGeochemistry"  ; 
	skos:definition   "a research initiative in which the object is to determine the presence of substances commonly found under the Earth's surface"  . 

c4p:forensicGeochemistry rdf:type skos:Concept ; 
	skos:prefLabel   "forensicGeochemistry"  ; 
	skos:definition   "a scientific methodology developed for identifying petroleum-related and other potentially hazardous environmental contaminants and for determining their sources and time of release"  . 

c4p:geochemistry rdf:type skos:Concept ; 
	skos:prefLabel   "geochemistry"  ; 
	skos:definition   "the study of the chemical composition of the Earth and its rocks and minerals"  . 

c4p:isotopicGeochemistry rdf:type skos:Concept ; 
	skos:prefLabel   "isotopicGeochemistry"  ; 
	skos:definition   "an aspect of geology based upon study of the natural variations in the relative abundances of isotopes of various elements."  . 

c4p:petroleumGeochemistry rdf:type skos:Concept ; 
	skos:prefLabel   "petroleumGeochemistry"  ; 
	skos:definition   " the application of chemical principles to the study of the origin, migration, accumulation, and alteration of petroleum...(John M. Hunt, 1979). Petroleum is generally considered oil and natural gases having various compounds composed of primarily hydrogen and carbon."  . 

c4p:regionalGeochemistry rdf:type skos:Concept ; 
	skos:prefLabel   "regionalGeochemistry"  ; 
	skos:definition   "the study of the spatial variation in the chemical composition of materials at the surface of the Earth, on a scale of tens to thousands of kilometres"  . 

c4p:terrestrialGeochemistry rdf:type skos:Concept ; 
	skos:prefLabel   "terrestrialGeochemistry"  ; 
	skos:definition   "the study of the chemical composition of the earth and its rocks and minerals"  . 

c4p:absoluteDating rdf:type skos:Concept ; 
	skos:prefLabel   "absoluteDating"  ; 
	skos:definition   "the process of determining an approximate computed age in archaeology and geology. Some scientists prefer the terms chronometric or calendar dating, as use of the word absolute implies an unwarranted certainty and precision."  . 

c4p:biostratigraphy rdf:type skos:Concept ; 
	skos:prefLabel   "biostratigraphy"  ; 
	skos:definition   "the branch of stratigraphy concerned with fossils and their use in dating rock formations."  . 

c4p:chronostratigraphy rdf:type skos:Concept ; 
	skos:prefLabel   "chronostratigraphy"  ; 
	skos:definition   "the branch of geology concerned with establishing the absolute ages of strata"  . 

c4p:geochronology rdf:type skos:Concept ; 
	skos:prefLabel   "geochronology"  ; 
	skos:definition   "the branch of geology concerned with the dating of rock formations and geological events"  . 

c4p:geochronometry rdf:type skos:Concept ; 
	skos:prefLabel   "geochronometry"  ; 
	skos:definition   "the measurement of geological time to produce a numerical time-scale (not `absolute', as there is always a margin of error). It applies geochronological methods, especially radiometric dating."  . 

c4p:geologicTime rdf:type skos:Concept ; 
	skos:prefLabel   "geologicTime"  ; 
	skos:definition   "Interval of time occupied by the Earth's geologic history, extending from c. 3.9 billion years ago (corresponding to the age of the oldest known rocks) to the present day."  . 

c4p:historicalGeology rdf:type skos:Concept ; 
	skos:prefLabel   "historicalGeology"  ; 
	skos:definition   " a discipline that uses the principles and techniques of geology to reconstruct and understand the geological history of Earth"  . 

c4p:isotopicGeochronology rdf:type skos:Concept ; 
	skos:prefLabel   "isotopicGeochronology"  ; 
	skos:definition   "the branch of geology concerned with the dating of rock formations and geological events using isotopic dating"  . 

c4p:lithostratigraphy rdf:type skos:Concept ; 
	skos:prefLabel   "lithostratigraphy"  ; 
	skos:definition   "a sub-discipline of stratigraphy, the geological science associated with the study of strata or rock layers. Major focuses include geochronology, comparative geology, and petrology. In general a stratum will be primarily igneous or sedimentary relating to how the rock was formed."  . 

c4p:relativeDating rdf:type skos:Concept ; 
	skos:prefLabel   "relativeDating"  ; 
	skos:definition   "the science of determining the relative order of past events, without necessarily determining their absolute age. In geology rock or superficial deposits, fossils and lithologies can be used to correlate one stratigraphic column with another"  . 

c4p:cartography rdf:type skos:Concept ; 
	skos:prefLabel   "cartography"  ; 
	skos:definition   "the science or practice of drawing maps"  . 

c4p:dataManipulation rdf:type skos:Concept ; 
	skos:prefLabel   "dataManipulation"  ; 
	skos:definition   "A data manipulation language is a family of syntax elements similar to a computer programming language used for selecting, inserting, deleting and updating data in a database"  . 

c4p:forcasting rdf:type skos:Concept ; 
	skos:prefLabel   "forcasting"  ; 
	skos:definition   "predict or estimate (a future event or trend)"  . 

c4p:geography rdf:type skos:Concept ; 
	skos:prefLabel   "geography"  ; 
	skos:definition   "the study of the physical features of the earth and its atmosphere, and of human activity as it affects and is affected by these, including the distribution of populations and resources, land use, and industries"  . 

c4p:geologicMapping rdf:type skos:Concept ; 
	skos:prefLabel   "geologicMapping"  ; 
	skos:definition   "A geologic map or geological map is a special-purpose map made to show geological features. Rock units or geologic strata are shown by color or symbols to indicate where they are exposed at the surface"  . 

c4p:geomodeling rdf:type skos:Concept ; 
	skos:prefLabel   "geomodeling"  ; 
	skos:definition   " the applied science of creating computerized representations of portions of the Earth's crust based on geophysical and geological observations made on and below the Earth surface."  . 

c4p:gIS rdf:type skos:Concept ; 
	skos:prefLabel   "gIS"  ; 
	skos:definition   "geographic information system (GIS) is a computer system designed to capture, store, manipulate, analyze, manage, and present all types of geographical data."  . 

c4p:graphing rdf:type skos:Concept ; 
	skos:prefLabel   "graphing"  ; 
	skos:definition   "plot or trace on a graph"  . 

c4p:lIDAR rdf:type skos:Concept ; 
	skos:prefLabel   "lIDAR"  ; 
	skos:definition   "a detection system that works on the principle of radar, but uses light from a laser"  . 

c4p:mapping rdf:type skos:Concept ; 
	skos:prefLabel   "mapping"  ; 
	skos:definition   "an operation that associates each element of a given set (the domain) with one or more elements of a second set (the range)"  . 

c4p:metadata rdf:type skos:Concept ; 
	skos:prefLabel   "metadata"  ; 
	skos:definition   "a set of data that describes and gives information about other data"  . 

c4p:modelling rdf:type skos:Concept ; 
	skos:prefLabel   "modelling"  ; 
	skos:definition   "a representation, generally in miniature, to show the construction or appearance of something"  . 

c4p:satellite rdf:type skos:Concept ; 
	skos:prefLabel   "satellite"  ; 
	skos:definition   "an artificial body placed in orbit around the earth or moon or another planet in order to collect information or for communication"  . 

c4p:statisticalAnalysis rdf:type skos:Concept ; 
	skos:prefLabel   "statisticalAnalysis"  ; 
	skos:definition   " refers to a collection of methods used to process large amounts of data and report overall trends. Statistical analysis is particularly useful when dealing with noisy data."  . 

c4p:visualization rdf:type skos:Concept ; 
	skos:prefLabel   "visualization"  ; 
	skos:definition   "the act or process of interpreting in visual terms or of putting into visible form"  . 

c4p:geohydrology rdf:type skos:Concept ; 
	skos:prefLabel   "geohydrology"  ; 
	skos:definition   "1. Hydrogeology (hydro- meaning water, and -geology meaning the study of the Earth) is the area of geology that deals with the distribution and movement of groundwater in the soil and rocks of the Earth's crust (commonly in aquifers). The term geohydrology is often used interchangeably."  . 

c4p:hydrogeology rdf:type skos:Concept ; 
	skos:prefLabel   "hydrogeology"  ; 
	skos:definition   "1. Hydrogeology (hydro- meaning water, and -geology meaning the study of the Earth) is the area of geology that deals with the distribution and movement of groundwater in the soil and rocks of the Earth's crust (commonly in aquifers). The term geohydrology is often used interchangeably."  . 

c4p:hydrology rdf:type skos:Concept ; 
	skos:prefLabel   "hydrology"  ; 
	skos:definition   "the branch of science concerned with the properties of the earth's water, especially its movement in relation to land"  . 

c4p:lacustrine rdf:type skos:Concept ; 
	skos:prefLabel   "lacustrine"  ; 
	skos:definition   "of, relating to, or associated with lakes"  . 

c4p:limnogeology rdf:type skos:Concept ; 
	skos:prefLabel   "limnogeology"  ; 
	skos:definition   " the study of lake systems and their deposits"  . 

c4p:limnology rdf:type skos:Concept ; 
	skos:prefLabel   "limnology"  ; 
	skos:definition   "the study of the biological, chemical, and physical features of lakes and other bodies of fresh water"  . 

c4p:bathymetry rdf:type skos:Concept ; 
	skos:prefLabel   "bathymetry"  ; 
	skos:definition   "the measurement of depth of water in oceans, seas, or lakes"  . 

c4p:deepSeaResearch rdf:type skos:Concept ; 
	skos:prefLabel   "deepSeaResearch"  ; 
	skos:definition   "research of the deep sea"  . 

c4p:marineGeoscience rdf:type skos:Concept ; 
	skos:prefLabel   "marineGeoscience"  ; 
	skos:definition   "the branch of geology dealing with the rocks, sediments, and processes of the floors and margins of the oceans"  . 

c4p:paleobathymetry rdf:type skos:Concept ; 
	skos:prefLabel   "paleobathymetry"  ; 
	skos:definition   " the study of past underwater depths"  . 

c4p:paleoceanography rdf:type skos:Concept ; 
	skos:prefLabel   "paleoceanography"  ; 
	skos:definition   " the study of the history of the oceans in the geologic past with regard to circulation, chemistry, biology, geology and patterns of sedimentation and biological productivity"  . 

c4p:paleomagnetism rdf:type skos:Concept ; 
	skos:prefLabel   "paleomagnetism"  ; 
	skos:definition   "the branch of geophysics concerned with the magnetism in rocks that was induced by the earth's magnetic field at the time of their formation"  . 

c4p:oceanography rdf:type skos:Concept ; 
	skos:prefLabel   "oceanography"  ; 
	skos:definition   "the branch of science that deals with the physical and biological properties and phenomena of the sea"  . 

c4p:biofacies rdf:type skos:Concept ; 
	skos:prefLabel   "biofacies"  ; 
	skos:definition   "a part of a stratigraphic unit in which the fossil fauna or flora differs significantly from that found elsewhere in the same unit"  . 

c4p:biostratinomy rdf:type skos:Concept ; 
	skos:prefLabel   "biostratinomy"  ; 
	skos:definition   " the study of the processes that take place after an organism dies but before its final burial. It is considered to be a subsection of the science of taphonomy, along with necrology (the study of the death of an organism) and diagenesis (the changes that take place after final burial)"  . 

c4p:calcareousNannofossil rdf:type skos:Concept ; 
	skos:prefLabel   "calcareousNannofossil"  ; 
	skos:definition   "Calcareous nannofossils include the coccoliths and coccospheres of haptophyte algae and the associated nannoliths which are of unknown provenance"  . 

c4p:fossilization rdf:type skos:Concept ; 
	skos:prefLabel   "fossilization"  ; 
	skos:definition   "To become a fossil"  . 

c4p:invertebrate rdf:type skos:Concept ; 
	skos:prefLabel   "invertebrate"  ; 
	skos:definition   "an animal lacking a backbone, such as an arthropod, mollusk, annelid, coelenterate, etc. The invertebrates constitute an artificial division of the animal kingdom, comprising 95 percent of animal species and about 30 different phyla"  . 

c4p:vertebrate rdf:type skos:Concept ; 
	skos:prefLabel   "vertebrate"  ; 
	skos:definition   "an animal of a large group distinguished by the possession of a backbone or spinal column, including mammals, birds, reptiles, amphibians, and fishes"  . 

c4p:geoarcheology rdf:type skos:Concept ; 
	skos:prefLabel   "geoarcheology"  ; 
	skos:definition   "a multi-disciplinary approach which uses the techniques and subject matter of geography, geology and other Earth sciences to examine topics which inform archaeological knowledge and thought."  . 

c4p:ichnology rdf:type skos:Concept ; 
	skos:prefLabel   "ichnology"  ; 
	skos:definition   "the study of plant and animal traces. Implicit to this definitionis that the traces made by plants and animals reflect some sort of behavior.Ichnology can be divided into two major subdivisions which are paleoichnology, the study of ancient traces and neoichnology, the study of modern traces"  . 

c4p:mammalPaleobiology rdf:type skos:Concept ; 
	skos:prefLabel   "mammalPaleobiology"  ; 
	skos:definition   "the branch of science concerned with fossil animals specifically mammals"  . 

c4p:microfossil rdf:type skos:Concept ; 
	skos:prefLabel   "microfossil"  ; 
	skos:definition   "a fossil or fossil fragment that can be seen only with a microscope"  . 

c4p:micropaleobiology rdf:type skos:Concept ; 
	skos:prefLabel   "micropaleobiology"  ; 
	skos:definition   "(also sometimes spelled as micropalaeontology) is the branch of palaeontology that studies microfossils. Microfossils[edit] Diatomaceous earth is a soft, siliceous, sedimentary rock made up of microfossils in the form of the frustules (shells) of single cell diatoms"  . 

c4p:morphology rdf:type skos:Concept ; 
	skos:prefLabel   "morphology"  ; 
	skos:definition   "the study of the forms of things, in particular"  . 

c4p:paleobiogeography rdf:type skos:Concept ; 
	skos:prefLabel   "paleobiogeography"  ; 
	skos:definition   "the study of the distribution of ancient plants and animals and their relation to ancient geographicfeatures"  . 

c4p:paleobiology rdf:type skos:Concept ; 
	skos:prefLabel   "paleobiology"  ; 
	skos:definition   "the biology of fossil animals and plants"  . 

c4p:paleobotany rdf:type skos:Concept ; 
	skos:prefLabel   "paleobotany"  ; 
	skos:definition   "the study of fossil plants"  . 

c4p:paleoecology rdf:type skos:Concept ; 
	skos:prefLabel   "paleoecology"  ; 
	skos:definition   "the ecology of fossil animals and plants"  . 

c4p:paleoentomology rdf:type skos:Concept ; 
	skos:prefLabel   "paleoentomology"  ; 
	skos:definition   "a branch of entomology that deals with fossil insects"  . 

c4p:paleofire rdf:type skos:Concept ; 
	skos:prefLabel   "paleofire"  ; 
	skos:definition   "fire history derived from natural proxies"  . 

c4p:paleoichthyology rdf:type skos:Concept ; 
	skos:prefLabel   "paleoichthyology"  ; 
	skos:definition   "The evolution of fish is not studied as a single event since fish do not represent a monophyletic group. Fish first appeared during the Cambrian explosion, around 530 million years ago."  . 

c4p:paleontology rdf:type skos:Concept ; 
	skos:prefLabel   "paleontology"  ; 
	skos:definition   "the branch of science concerned with fossil animals and plants"  . 

c4p:paleozoology rdf:type skos:Concept ; 
	skos:prefLabel   "paleozoology"  ; 
	skos:definition   "the branch of paleontology dealing with fossil animals. The scientific study of animal fossils and the evolution of animals"  . 

c4p:palynology rdf:type skos:Concept ; 
	skos:prefLabel   "palynology"  ; 
	skos:definition   "the study of pollen grains and other spores, especially as found in archaeological or geological deposits"  . 

c4p:taphonomy rdf:type skos:Concept ; 
	skos:prefLabel   "taphonomy"  ; 
	skos:definition   "the branch of paleontology that deals with the processes of fossilization"  . 

c4p:drilling rdf:type skos:Concept ; 
	skos:prefLabel   "drilling"  ; 
	skos:definition   "produce (a hole) in something by or as if by boring with a drill"  . 

c4p:economicGeology rdf:type skos:Concept ; 
	skos:prefLabel   "economicGeology"  ; 
	skos:definition   "a specialty within geology--not within economics--that is concerned with earth materials that are, or can be potentially, economically utilized by society. This includes metals, nonmetallic minerals, rocks, fuels, and water."  . 

c4p:energyResources rdf:type skos:Concept ; 
	skos:prefLabel   "energyResources"  ; 
	skos:definition   "energy that comes fromresources which are naturally replenished on a human timescale such as sunlight, wind, rain, tides, waves and geothermal heat"  . 

c4p:geodesy rdf:type skos:Concept ; 
	skos:prefLabel   "geodesy"  ; 
	skos:definition   "the branch of mathematics dealing with the shape and area of the earth or large portions of it"  . 

c4p:engineeringGeology rdf:type skos:Concept ; 
	skos:prefLabel   "engineeringGeology"  ; 
	skos:definition   "the application of geological data, techniques and principles to the study of rock and soil surficial materials, and ground water. This is essential for the proper location, planning, design, construction, operation and maintenance of engineering structures"  . 

c4p:geophysics rdf:type skos:Concept ; 
	skos:prefLabel   "geophysics"  ; 
	skos:definition   "the physics of the earth"  . 

c4p:mineralogy rdf:type skos:Concept ; 
	skos:prefLabel   "mineralogy"  ; 
	skos:definition   "the scientific study of minerals"  . 

c4p:miningGeology rdf:type skos:Concept ; 
	skos:prefLabel   "miningGeology"  ; 
	skos:definition   "an applied science which combines the principles of economic geology and mining engineering to the development of a defined mineral resource. Mining geologists and engineers work to develop an identified ore deposit to economically extract the ore"  . 

c4p:naturalResources rdf:type skos:Concept ; 
	skos:prefLabel   "naturalResources"  ; 
	skos:definition   "materials or substances such as minerals, forests, water, and fertile land that occur in nature and can be used for economic gain"  . 

c4p:ore rdf:type skos:Concept ; 
	skos:prefLabel   "ore"  ; 
	skos:definition   "a naturally occurring solid material from which a metal or valuable mineral can be profitably extracted"  . 

c4p:petroleumGeology rdf:type skos:Concept ; 
	skos:prefLabel   "petroleumGeology"  ; 
	skos:definition   " the study of origin, occurrence, movement, accumulation, and exploration of hydrocarbon fuels. It refers to the specific set of geological disciplines that are applied to the search for hydrocarbons (oil exploration)"  . 

c4p:petrology rdf:type skos:Concept ; 
	skos:prefLabel   "petrology"  ; 
	skos:definition   "the branch of science concerned with the origin, small-scale structure, and composition of rocks"  . 

c4p:petrophysics rdf:type skos:Concept ; 
	skos:prefLabel   "petrophysics"  ; 
	skos:definition   "the branch of geology concerned with the physical properties and behavior of rocks"  . 

c4p:seismology rdf:type skos:Concept ; 
	skos:prefLabel   "seismology"  ; 
	skos:definition   "the branch of science concerned with earthquakes and related phenomena"  . 

c4p:subsurfaceExploration rdf:type skos:Concept ; 
	skos:prefLabel   "subsurfaceExploration"  ; 
	skos:definition   "The physical process of probing the geophysical subsurface in order to determine the structure and/or the presence of anomalies"  . 

c4p:tectonics rdf:type skos:Concept ; 
	skos:prefLabel   "tectonics"  ; 
	skos:definition   "large-scale processes affecting the structure of the earth's crust"  . 

c4p:coastalSedimentology rdf:type skos:Concept ; 
	skos:prefLabel   "coastalSedimentology"  ; 
	skos:definition   "Scientific discipline concerned with the physical and chemical properties of coastal sedimentary rocks and the processes involved in their formation, including transportation, deposition, and lithification of sediments."  . 

c4p:edaphology rdf:type skos:Concept ; 
	skos:prefLabel   "edaphology"  ; 
	skos:definition   "is concerned with the influence of soils on living things, particularly plants."  . 

c4p:paleomagnetism rdf:type skos:Concept ; 
	skos:prefLabel   "paleomagnetism"  ; 
	skos:definition   "the branch of geophysics concerned with the magnetism in rocks that was induced by the earth's magnetic field at the time of their formation"  . 

c4p:pedology rdf:type skos:Concept ; 
	skos:prefLabel   "pedology"  ; 
	skos:definition   "another term for soil science"  . 

c4p:relativeDating rdf:type skos:Concept ; 
	skos:prefLabel   "relativeDating"  ; 
	skos:definition   "the science of determining the relative order of past events, without necessarily determining their absolute age. In geology rock or superficial deposits, fossils and lithologies can be used to correlate one stratigraphic column with another"  . 

c4p:sedimentology rdf:type skos:Concept ; 
	skos:prefLabel   "sedimentology"  ; 
	skos:definition   "Scientific discipline concerned with the physical and chemical properties of sedimentary rocks and the processes involved in their formation, including transportation, deposition, and lithification of sediments"  . 

c4p:stratigraphy rdf:type skos:Concept ; 
	skos:prefLabel   "stratigraphy"  ; 
	skos:definition   "the branch of geology concerned with the order and relative position of strata and their relationship to the geological time scale; the analysis of the order and position of layers of archaeological remains; the structure of a particular set of strata"  . 

